it's all over :)

theories/pop_corr.v
@@ -8,7 +8,7 @@ From AAC_tactics Require Import AAC.
 From AAC_tactics Require Import Instances.
 Import Instances.Lists.
 
-From Deque Require Import common tick shared_ref deque_corr eject_corr_lemmas.
+From Deque Require Import common tick shared_ref deque_corr push_corr concat_corr pop_corr_lemmas.
 
 Section proof.
 
@@ -18,74 +18,72 @@ Section proof.
   Let TIME_CHEAT : ∀ k, ⊢ (⏱ k : iProp Σ).
   Admitted.
 
-  Lemma eject_spec_helper oD x (ℓ : loc) :
-    {{{ isDeque (oD ++ ⋅x) (SOMEV #ℓ) }}}
-      eject_nonempty (#ℓ)
-    {{{ d', RET (d', x)%V; isDeque oD d' }}}.
+  Lemma pop_spec_helper oD x (ℓ : loc) :
+    {{{ isDeque (⋅x ++ oD) (SOMEV #ℓ) }}}
+      pop_nonempty (#ℓ)
+    {{{ d', RET (x, d')%V; isDeque oD d' }}}.
   Proof.
-    Transparent fiveTuple.
-    Opaque isEjectFiveTuple isUnsafeEjectFiveTuple prepare_eject naive_eject.
+    Opaque isPopFiveTuple isUnsafePopFiveTuple prepare_pop naive_pop.
     iIntros (ψ) "Hd Hψ".
     rewrite isDeque_unfold.
-    rewrite /eject_nonempty.
-    Opaque eject_nonempty.
+    rewrite /pop_nonempty.
+    Opaque pop_nonempty.
     iLöb as "iH" forall (ℓ oD x ψ).
     iDestruct "Hd" as "[[%H _] | (%ℓ' & %Heqℓ & #Hℓ)]". by inversion H.
     inversion Heqℓ as [H]. rewrite -H. clear Heqℓ H ℓ'.
     wp_pures.
-    iDestruct (TIME_CHEAT _) as "ι".
+    iDestruct (TIME_CHEAT) as "ι".
     wp_apply (tick_spec with "ι") as "_".
     wp_pures.
-    wp_apply (csref_load with "[Hℓ]") as (d) "πd". by apply fiveTuplePersistent.
-      by iExact "Hℓ".
-    iDestruct (safe_decidable (oD++⋅x) d with "πd") as "[Unsafe | Safe]".
+    wp_apply (csref_load with "Hℓ") as (d) "πd".
+    iDestruct (safe_decidable (⋅x ++ oD) d with "πd") as "[Unsafe | Safe]".
     wp_pures.
     2: {
       wp_pures.
-      iDestruct "Safe" as "(Hsafe & eject_safe)".
+      iDestruct "Safe" as "(Hsafe & pop_safe)".
       iDestruct "Hsafe" as "#Hsafe".
-      iAssert (fiveTuple (oD ++ ⋅x) d) as "Hd".
-      - Transparent isEjectFiveTuple.
+      iAssert (fiveTuple (⋅x ++ oD) d) as "Hd".
+      - Transparent isPopFiveTuple.
         iDestruct "Hsafe" as "(%p & %l & %m & %r & %s & %op & %ol & %om & %or & %os &
                             %kPr & %kMd & %kSf & %ltr & %rtr &
                             -> & %conf & #Hp & #Hl & #Hm & #Hr & #Hs &
                             #Hltr & #Hrtr & %Hoeq)".
-        Opaque isEjectFiveTuple.
+        Opaque isPopFiveTuple.
         iExists p, l, m, r, s, op, ol, om, or, os, kPr, kMd, kSf, ltr, rtr.
         doneL.
         iSplit. iPureIntro. inversion conf; by easy_config.
         iFrame "#". iFrame.
         done.
-      - wp_bind (naive_eject_safe d)%E.
-        iApply (wp_wand with "eject_safe").
+      - wp_bind (naive_pop_safe d)%E.
+        iApply (wp_wand with "pop_safe").
         iIntros (true_) "->".
         Opaque fiveTuple.
         wp_pures.
-        wp_bind (#ℓ <- d)%E.
-        wp_apply (csref_store with "[Hℓ]") as "_".
+        wp_apply (csref_store with "[Hℓ]").
         {
           iSplit. iExact "Hℓ".
           by iFrame.
         }
-        wp_pures.
-        wp_apply (safe_naive_eject) as (x' d' o') "(Hd' & %Heq)".
-          { iFrame "#".
-          }
-        destruct (app_sing_inv _ _ _ _ Heq) as [-> ->].
+        iIntros (unit).
+        wp_pures; clear unit.
+        wp_apply (safe_naive_pop with "[Hd]") as (x' d' o') "(Hd' & %Heq)".
+        { iFrame "#".
+        }
+        inversion Heq.
         iApply "Hψ".
         by iFrame.
       Transparent fiveTuple.
     }
-    iDestruct "Unsafe" as "[Hunsafe eject_unsafe]".
-    wp_bind (naive_eject_safe d)%E.
-    iApply (wp_wand with "eject_unsafe").
+    iDestruct "Unsafe" as "[Hunsafe pop_unsafe]".
+    wp_bind (naive_pop_safe d)%E.
+    iApply (wp_wand with "pop_unsafe").
     iIntros (false_) "->".
     wp_pures.
-    wp_apply (prepare_eject_spec with "[Hunsafe]").
+    wp_apply (prepare_pop_spec with "[Hunsafe]").
     - iFrame.
       iIntros (ℓ' x' o') "Hℓ'".
-      Transparent eject_nonempty.
-      rewrite /eject_nonempty.
+      Transparent pop_nonempty.
+      rewrite /pop_nonempty.
       iApply ("iH" with "[Hℓ']"); iClear "iH"; try done.
       + rewrite -isDeque_unfold. ℓisDeque ℓ'. iExact "Hℓ'".
       + iNext.
@@ -94,24 +92,24 @@ Section proof.
     - iIntros (f') "Hf'". iClear "iH".
       wp_pures.
       wp_bind (#ℓ <- f')%E.
-      Transparent isEjectFiveTuple.
+      Transparent isPopFiveTuple.
       iDestruct "Hf'" as "(%p & %l & %m & %r & %s & %op & %ol & %om & %or & %os &
-                          %kp & %kMd & %ks & %ltr & %rtr &
+                          %kPr & %kMd & %kSf & %ltr & %rtr &
                           -> & %conf & #Hp & #Hl & #Hm & #Hr & #Hs &
                           #Hltr & #Hrtr & %Hoeq)".
       wp_apply (csref_store with "[Hℓ]").
       {
         iSplit. iExact "Hℓ".
-        iExists p, l, m, r, s, op, ol, om, or, os, kp, kMd, ks, ltr, rtr.
+        iExists p, l, m, r, s, op, ol, om, or, os, kPr, kMd, kSf, ltr, rtr.
         doneL.
         iSplit. iPureIntro. inversion conf; by easy_config.
         iFrame "#". iFrame.
         done.
       }
-      iIntros "_". wp_pures.
-      wp_apply (safe_naive_eject).
+      iIntros (unit). wp_pures; clear unit.
+      wp_apply (safe_naive_pop).
       + iFrame.
-        iExists p, l, m, r, s, op, ol, om, or, os, kp, kMd, ks, ltr, rtr.
+        iExists p, l, m, r, s, op, ol, om, or, os, kPr, kMd, kSf, ltr, rtr.
         doneL.
         iSplit. iPureIntro. inversion conf; by easy_config.
         iFrame "#". iFrame.
@@ -119,25 +117,25 @@ Section proof.
         iSplit. iApply (big_sepL2_mono with "Hrtr"). by auto.
         done.
       + iIntros (x' d' o') "[Hd %Heq]".
-        destruct (app_sing_inv _ _ _ _ Heq) as [-> ->].
+        inversion Heq.
         iApply "Hψ".
         iFrame.
   Qed.
 
-  Definition eject_spec : forall x o d,
-    {{{ IsDeque (o++⋅x) d }}}
-      eject d
-    {{{ d', RET (d', x)%V; IsDeque o d' }}}.
+  Definition pop_spec : forall x o d,
+    {{{ IsDeque (⋅x ++ o) d }}}
+      pop d
+    {{{ d', RET (x, d')%V; IsDeque o d' }}}.
   Proof.
     iIntros (x o d ψ) "#Hd hψ".
-    rewrite /eject.
+    rewrite /pop.
     wp_pures.
     rewrite /IsDeque isDeque_unfold.
     iCombine "Hd Hd" as "[_ [[-> %Heq]|(%ℓ & -> & Hℓ)]]";
       rewrite -isDeque_unfold;
-      [ destruct o; simpl in Heq; inversion Heq |].
+      [ inversion Heq |].
     wp_pures.
-    wp_apply (eject_spec_helper).
+    wp_apply (pop_spec_helper).
       by (iFrame; iFrame "#").
     done.
   Qed.
