theories/concat_corr.v
@@ -1,0 +1,350 @@
+From iris.heap_lang Require Import lang proofmode notation.
+From iris.bi Require Import derived_laws.
+
+From Coq Require Import List.
+Import ListNotations.
+
+From AAC_tactics Require Import AAC.
+From AAC_tactics Require Import Instances.
+Import Instances.Lists.
+
+From Deque Require Import common tick shared_ref deque_corr push_corr inject_corr.
+
+Section proof.
+
+  Context `{!heapGS Σ}.
+
+  (* since this is a functional correction proof, we use a cheat that is confined to this section *)
+  Let TIME_CHEAT : ∀ k, ⊢ (⏱ k : iProp Σ).
+  Admitted.
+
+  Lemma safe_inject_whole :
+    ∀ sC dC d, isDeque dC d -∗
+    fold.safe_fold id inject d sC (isDeque (dC ++ sC)).
+  Proof.
+    intro.
+    iInduction sC as [| x sC ].
+    all: iIntros (dC d) "#Hd".
+    all: rewrite /fold.safe_fold.
+    - iFrame. rewrite app_nil_r //.
+    - iApply (inject_spec_helper).
+        { iFrame. iExact "Hd". }
+      iNext.
+      iIntros (d') "Hd'".
+      iSpecialize ("IHsC").
+      iSpecialize ("IHsC" $! (dC ++ ⋅x) d' with "Hd'").
+      assert (dC ++ x :: sC = ((dC ++ [x]) ++ sC)) as ->
+        by rewrite cons_middle app_assoc //.
+      done.
+  Qed.
+
+  Lemma inject_whole_spec : forall s d k sC dC,
+    {{{ buffer k sC s ∗ isDeque dC d }}}
+      bfold_left inject d s
+    {{{ d', RET d'; isDeque (dC ++ sC) d' }}}.
+  Proof.
+    intros. iIntros "(#Hs & #Hd) Hϕ".
+    wp_apply (bfold_left_spec _ _ _ _ (isDeque (dC ++ sC))%I).
+    - iFrame "#".
+      iDestruct (buffer_length with "Hs") as "<-".
+      by iApply (safe_inject_whole sC).
+    - by iApply "Hϕ".
+  Qed.
+
+  Lemma safe_push_whole :
+    ∀ sC dC d, isDeque dC d -∗
+    fold.safe_fold fold.fflip push d (rev sC) (isDeque (sC ++ dC)).
+  Proof.
+    intro.
+    rewrite -{2}(rev_involutive sC).
+    set (l := rev sC).
+    assert (l = rev sC) by done.
+    move: sC l H => sC l.
+    move: l sC => l.
+    iInduction l as [| x l].
+    all: iIntros (sC Heq dC d) "#Hd".
+    - iFrame.
+      rewrite //.
+    - rewrite /fold.safe_fold.
+      wp_pures.
+      iApply (push_spec_helper).
+        { iFrame. iExact "Hd". }
+      iNext.
+      iIntros (d') "Hd'".
+      assert (l = rev (rev l)) as Hinv by rewrite rev_involutive //.
+      iSpecialize ("IHl" $! (rev l) Hinv).
+      iSpecialize ("IHl" $! (⋅x ++ dC) d' with "Hd'").
+      assert (rev (x::l) ++ dC = rev l ++ ⋅x ++ dC) as ->.
+        { assert (x::l = ⋅x ++ l) as -> by rewrite //.
+          rewrite rev_app_distr.
+          assert (rev [x] = [x]) as -> by rewrite //.
+          aac_reflexivity. }
+      done.
+  Qed.
+
+ Lemma push_whole_spec : forall s d k sC dC,
+    {{{ buffer k sC s ∗ isDeque dC d }}}
+      bfold_right push s d
+    {{{ d', RET d'; isDeque (sC ++ dC) d' }}}.
+  Proof.
+    intros. iIntros "(#Hs & #Hd) Hϕ".
+    wp_apply (bfold_right_spec _ _ _ _ (isDeque (sC ++ dC))%I).
+    - iFrame "#".
+      iDestruct (buffer_length with "Hs") as "<-".
+      by iApply (safe_push_whole sC).
+    - by iApply "Hϕ".
+  Qed.
+
+  Theorem dconcat_spec_helper (d1 d2 : val) : forall o1 o2,
+    {{{ isDeque o1 d1 ∗ isDeque o2 d2 }}}
+      dconcat d1 d2
+    {{{ d', RET d'; isDeque (o1 ++ o2) d' }}}.
+  Proof.
+    iIntros (o1 o2 ψ) "(Hd1 & Hd2) Hψ".
+    rewrite /dconcat /IsDeque.
+    wp_pures.
+    iDestruct (TIME_CHEAT 1) as "ι".
+    wp_apply (tick_spec with "ι") as "_".
+    wp_pures.
+    (* trivial cases *)
+    rewrite {1} isDeque_unfold.
+    iDestruct "Hd1" as "[[-> ->] | (%ℓ1 & -> & #Hℓ1)]".
+    { wp_pures. iApply "Hψ". rewrite app_nil_l //. }
+    rewrite {1} isDeque_unfold.
+    iDestruct "Hd2" as "[[-> ->] | (%ℓ2 & -> & #Hℓ2)]".
+    { wp_pures. iApply "Hψ". iFrame. ℓisDeque ℓ1. rewrite app_nil_r. iExact "Hℓ1". }
+    wp_pures.
+    wp_apply (csref_load with "Hℓ1") as "%v
+      (%pr1 & %ld1 & %md1 & %rd1 & %sf1 & %prC1 & %ldC1 & %mdC1 & %rdC1 & %sfC1
+            & %kPr1 & %kMd1 & %kSf1 & %ltr1 & %rtr1 & -> & %cfg1
+            & #Hpr1 & #Hld1 & #Hmd1 & #Hrd1 & #Hsf1 & #Hltr1 & #Hrtr1 & %Heq1)
+      ".
+    wp_pures.
+    wp_apply (csref_load with "Hℓ2") as "%v'
+      (%pr2 & %ld2 & %md2 & %rd2 & %sf2 & %prC2 & %ldC2 & %mdC2 & %rdC2 & %sfC2
+            & %kPr2 & %kMd2 & %kSf2 & %ltr2 & %rtr2 & -> & %cfg2
+            & #Hpr2 & #Hld2 & #Hmd2 & #Hrd2 & #Hsf2 & #Hltr2 & #Hrtr2 & %Heq2)
+      ".
+    wp_pures.
+    wp_apply (bis_empty_spec with "Hmd1") as "_".
+    wp_pures.
+    destruct (bool_decide (kMd1 = 0)) eqn:?.
+    { (* d1 is suffix only *)
+      apply bool_decide_eq_true_1 in Heqb as Heqmd.
+      inversion cfg1; [| exfalso; lia].
+      wp_pures.
+      wp_apply (push_whole_spec).
+      - iFrame "#". iFrame.
+        ℓisDeque ℓ2. iExact "Hℓ2".
+      - iDestruct (buffer_length with "Hpr1") as "%Hpr1L";
+          destruct prC1; [| inversion Hpr1L].
+        iDestruct (buffer_length with "Hmd1") as "%Hmd1L";
+          destruct mdC1; [| inversion Hmd1L].
+        rewrite (nil_length_inv _ (eq_sym H)) in Heq1 |- *.
+        rewrite (nil_length_inv _ (eq_sym H1)) in Heq1 |- *.
+        aac_normalise in Heq1.
+        rewrite Heq1.
+        by iApply "Hψ".
+      }
+    apply bool_decide_eq_false_1 in Heqb as Heqmd1.
+    wp_pures.
+    wp_apply (bis_empty_spec with "Hmd2") as "_".
+    wp_pures.
+    destruct (bool_decide (kMd2 = 0)) eqn:?.
+    { (* d2 is suffix only *)
+      apply bool_decide_eq_true_1 in Heqb0 as Heqmd.
+      inversion cfg2; [| exfalso; lia].
+      wp_pures.
+      wp_apply (inject_whole_spec).
+      - iFrame "#". iFrame.
+        ℓisDeque ℓ1. iExact "Hℓ1".
+      - iDestruct (buffer_length with "Hpr2") as "%Hpr2L";
+          destruct prC2; [| inversion Hpr2L].
+        iDestruct (buffer_length with "Hmd2") as "%Hmd2L";
+          destruct mdC2; [| inversion Hmd2L].
+        rewrite (nil_length_inv _ (eq_sym H)) in Heq2 |- *.
+        rewrite (nil_length_inv _ (eq_sym H1)) in Heq2 |- *.
+        aac_normalise in Heq2.
+        rewrite Heq2.
+        by iApply "Hψ".
+    }
+    apply bool_decide_eq_false_1 in Heqb0 as Heqmd2.
+    wp_pures.
+    inversion cfg1; [exfalso; by apply Heqmd2 |].
+    inversion cfg2; [exfalso; by apply Heqmd2 |].
+    change (kSf1 ∈ map S [2; 3; 4; 5]) in H0.
+    apply decrease_in in H0 as (kSf1' & -> & HkSf1').
+    wp_apply (beject_spec with "Hsf1") as "%sf1' %x %oBX (Hsf1' & ->)".
+    wp_pures.
+    change (kPr2 ∈ map S [2; 3; 4; 5]) in H6.
+    apply decrease_in in H6 as (kPr2' & -> & HkPr2').
+    wp_apply (bpop_spec with "Hpr2") as "%y %pr1' %oBY (Hpr2' & ->)".
+    wp_pures.
+    wp_apply (bdoubleton_spec) as "%md' #Hmd'". { done. }
+    wp_pures.
+    wp_apply (bsplit23l_spec with "[Hsf1']") as "%s1' %s1'' %os1' %os1'' %ks1' %ks1'' (#Hs1' & #Hs1'' & (%Hks1' & %Hks1'' & %Heqos1))".
+      { iFrame. iPureIntro. invert_all_in; list_elem_of. }
+    rewrite /atriple_.
+    wp_pures.
+    wp_apply (inject_spec_helper with "Hld1") as "%ld1' #Hld1'".
+    wp_pures.
+    wp_bind (if: _ then _ else _)%E.
+    wp_apply (wp_strong_mono _ _ _ _ _
+      (λ v, ∃ tr trC, isDeque tr v ∗
+        ⌜ List.concat trC = List.concat ldC1 ++ mdC1 ++ List.concat rdC1 ++ os1' ++ os1'' ⌝ ∗
+        ([∗list] a;b ∈ trC; tr, ▷ triple a b))%I
+      ) as "%ld1'' (%tr1' & %trC1' & #Hld1'' & %HtrC1' & #trtrC1')"; try done.
+    {
+     wp_apply (bis_empty_spec with "Hs1''") as "_".
+      wp_pures.
+      destruct (bool_decide (ks1'' = 0)) eqn:?.
+      - apply bool_decide_eq_true_1 in Heqb1 as Heqs1.
+        wp_pures.
+        rewrite Heqs1.
+        iDestruct (buffer_length with "Hs1''") as "%Hs1''L".
+        destruct os1''; [| inversion Hs1''L].
+        rewrite !app_nil_r.
+        iExists (ltr1 ++ ⋅(md1, rd1, s1')%V), (ldC1 ++ ⋅(mdC1 ++ List.concat rdC1 ++ os1')).
+        iFrame "#". iFrame.
+        iModIntro.
+        iSplitL.
+        + iPureIntro. rewrite !concat_app /= app_nil_r //.
+        + iApply (big_sepL2_app with "[Hltr1]").
+          * iApply (big_sepL2_mono with "Hltr1"). by auto.
+          * simpl. doneR. iNext.
+            rewrite triple_unfold.
+            iExists md1, rd1, s1', mdC1, rdC1, os1', kMd1, ks1', rtr1.
+            inversion cfg1; [ rewrite -H3 in H14; lia |].
+            iSplitR. iPureIntro.
+            destruct (length rdC1); [apply left_leaning | apply has_child];
+              auto with arith; try list_elem_of.
+            iSplitR. done.
+            iFrame "#".
+            doneR.
+            iApply (big_sepL2_mono with "Hrtr1"). by auto.
+      - apply bool_decide_eq_false_1 in Heqb1 as Heqs1.
+        wp_pures.
+        wp_apply (abuffer_spec with "Hs1''") as "%ts1'' #Hts1''".
+          { inversion Hks1''; [lia | list_elem_of]. }
+        wp_apply (inject_spec_helper with "Hld1'") as "%ld1'' #Hld1''".
+        iExists ((ltr1 ++ ⋅(md1, rd1, s1')%V) ++ ⋅ts1''%V),
+                ((ldC1 ++ ⋅(mdC1 ++ List.concat rdC1 ++ os1')) ++ ⋅os1'').
+        iFrame. iFrame "#".
+        iSplitL.
+        + iPureIntro. rewrite /= !concat_app /=. aac_reflexivity.
+        + doneR.
+          iApply (big_sepL2_app with "[Hltr1]").
+          * iApply (big_sepL2_mono with "Hltr1"). by auto.
+          * simpl. doneR.
+            iNext.
+            rewrite !triple_unfold.
+            iExists md1, rd1, s1', mdC1, rdC1, os1', kMd1, ks1', rtr1.
+            inversion cfg1; [ rewrite -H3 in H14; lia |].
+            iSplitR. iPureIntro.
+            destruct (length rdC1); [apply left_leaning | apply has_child];
+              auto with arith; list_elem_of.
+            iSplitR. done.
+            iFrame "#".
+            doneR.
+            iApply (big_sepL2_mono with "Hrtr1"). by auto.
+    }
+    iModIntro. wp_pures.
+    wp_apply (bsplit23r_spec with "[Hpr2']") as "%p2' %p2'' %op2' %op2'' %kp2' %kp2'' (#Hp2' & #Hp2'' & (%Hp21' & %Hp2'' & %Hop2eq))".
+      { iFrame. iPureIntro. clear HkSf1' Hks1' Hks1''. invert_all_in; list_elem_of. }
+    wp_pures.
+    wp_apply (push_spec_helper with "Hrd2") as "%rd2' #Hrd2'".
+    wp_pures.
+    wp_bind (if: _ then _ else _)%E.
+    wp_apply (wp_strong_mono _ _ _ _ _
+      (λ v, ∃ tr trC, isDeque tr v ∗
+        ⌜ List.concat trC = op2' ++ op2'' ++ List.concat ldC2 ++ mdC2 ++ List.concat rdC2 ⌝ ∗
+        ([∗list] a;b ∈ trC; tr, ▷ triple a b))%I
+      ) as "%rd2'' (%tr2' & %trC2' & #Hrd2'' & %HtrC2' & #trtrC2')"; try done.
+    {
+      wp_apply (bis_empty_spec with "Hp2'") as "_".
+      wp_pures.
+      destruct (bool_decide (kp2' = 0)) eqn:?.
+      + apply bool_decide_eq_true_1 in Heqb1 as Heqp2.
+        wp_pures.
+        iFrame.
+        rewrite Heqp2.
+        iDestruct (buffer_length with "Hp2'") as "%Hp2'L".
+        destruct op2'; [| inversion Hp2'L].
+        rewrite !app_nil_l.
+        iExists (⋅(p2'', ld2, md2)%V ++ rtr2), (⋅(op2'' ++ List.concat ldC2 ++ mdC2) ++ rdC2).
+        iFrame "#".
+        iSplitR.
+        * iPureIntro. rewrite !concat_app /=. aac_reflexivity.
+        * simpl.
+          iSplitR.
+          -- iModIntro. iNext.
+            rewrite triple_unfold.
+            iExists p2'', ld2, md2, op2'', ldC2, mdC2, kp2'', kMd2, ltr2.
+            inversion cfg2.
+            { iDestruct (buffer_length with "Hpr2") as "%Habsurd". inversion Habsurd. }
+            iSplitR. iPureIntro.
+            destruct (length ldC2); [apply left_leaning | apply has_child];
+              try lia; list_elem_of.
+            iSplitR. done.
+            iFrame "#".
+            doneR.
+            iApply (big_sepL2_mono with "Hltr2"). by auto.
+          -- iApply (big_sepL2_mono with "Hrtr2"). by auto.
+      + apply bool_decide_eq_false_1 in Heqb1 as Heqp2.
+        wp_pures.
+        wp_apply (abuffer_spec with "Hp2'") as "%tp2' #Htp2'".
+          { inversion Hp21'; [lia | list_elem_of]. }
+        wp_apply (push_spec_helper with "Hrd2'") as "%rd2'' #Hrd2''".
+        iFrame.
+        iExists (⋅tp2' ++ ⋅(p2'', ld2, md2)%V ++ rtr2),
+                (⋅op2' ++ ⋅(op2'' ++ concat ldC2 ++ mdC2) ++ rdC2).
+        iFrame "#".
+        iSplitL.
+        * iPureIntro. rewrite !concat_app /=. aac_reflexivity.
+        * doneL.
+          iApply (big_sepL2_app with "[Hrtr2]").
+          -- simpl. doneR.
+            iNext.
+            rewrite !triple_unfold.
+            iExists p2'', ld2, md2, op2'', ldC2, mdC2, kp2'', kMd2, ltr2.
+            inversion cfg2.
+            { iDestruct (buffer_length with "Hpr2") as "%Habsurd". inversion Habsurd. }
+            iSplitR. iPureIntro.
+            destruct (length ldC2); [apply left_leaning | apply has_child];
+              auto with arith; list_elem_of.
+            iSplitR. done.
+            iFrame "#".
+            doneR.
+            iApply (big_sepL2_mono with "Hltr2"). by auto.
+          -- iApply (big_sepL2_mono with "Hrtr2"). by auto.
+    }
+    rewrite /assemble_.
+    iModIntro. wp_pures.
+    wp_apply (csref_alloc (fiveTuple (o1 ++ o2))) as (ℓ') "Hℓ'".
+    { iExists pr1, ld1'', md', rd2'', sf2,
+      prC1, trC1', (⋅oBX ++ ⋅pr1'), trC2', sfC2,
+      kPr1, 2, kSf2, tr1', tr2'.
+      iSplitR. done.
+      iSplitR. iPureIntro. constructor; list_elem_of.
+      iFrame "#".
+      iSplitL. iApply (big_sepL2_mono with "trtrC1'"). by auto.
+      iSplitL. iApply (big_sepL2_mono with "trtrC2'"). by auto.
+      iPureIntro.
+      rewrite Heq1 Heq2 Heqos1 Hop2eq HtrC1' HtrC2'.
+      aac_reflexivity.
+    }
+    wp_pures.
+    iApply "Hψ".
+    iFrame.
+    ℓisDeque ℓ'. iExact "Hℓ'".
+    Unshelve. all: by auto.
+  Qed.
+
+  Definition dconcat_spec d1 d2 : forall o1 o2,
+    {{{ isDeque o1 d1 ∗ isDeque o2 d2 }}}
+      dconcat d1 d2
+    {{{ d', RET d'; IsDeque (o1 ++ o2) d' }}}
+  :=
+    dconcat_spec_helper d1 d2.
+
+End proof.
