theories/pop_corr_lemmas.v
@@ -1,0 +1,1220 @@
+From iris.heap_lang Require Import lang proofmode notation.
+From iris.bi Require Import derived_laws.
+
+From Coq Require Import List.
+Import ListNotations.
+
+From AAC_tactics Require Import AAC.
+From AAC_tactics Require Import Instances.
+Import Instances.Lists.
+
+From Deque Require Import common tick shared_ref deque_corr push_corr concat_corr.
+
+Section lemmas.
+
+  Context `{!heapGS Σ}.
+
+  (* since this is a functional correction proof, we use a cheat that is confined to this section *)
+  Let TIME_CHEAT : ∀ k, ⊢ (⏱ k : iProp Σ).
+  Admitted.
+
+  (* Five-tuple configuration for calling naive_pop *)
+  Inductive pop_configuration : nat -> nat -> nat -> nat -> nat -> Prop :=
+    | pop_suffix_only : forall s, s ∈ [1..8] -> pop_configuration 0 0 0 0 s
+    | pop_has_middle : forall p ld rd s, p ∈ [4..6] -> s ∈ [3..6] -> pop_configuration p ld 2 rd s.
+
+ Definition isPopFiveTuple := (
+    λ o d, ∃ (pr ld md rd sf : val)
+      pr_content left_content md_content right_content sf_content
+      (kPr kMd kSf : nat) left_triples right_triples,
+      ⌜ d = (pr, ld, md, rd, sf)%V ⌝ ∗
+      ⌜ pop_configuration kPr (length left_content) kMd (length right_content) kSf ⌝ ∗
+      buffer kPr pr_content pr ∗
+      isDeque left_triples ld ∗
+      buffer kMd md_content md ∗
+      isDeque right_triples rd ∗
+      buffer kSf sf_content sf ∗
+      ([∗list] c;tr ∈ left_content;left_triples, ▷ triple c tr) ∗
+      ([∗list] c;tr ∈ right_content;right_triples, ▷ triple c tr) ∗
+      ⌜ o = pr_content ++ List.concat left_content ++ md_content ++ List.concat right_content ++ sf_content ⌝
+  )%I.
+
+ Definition isUnsafePopFiveTuple := (
+    λ o d, ∃ (pr ld md rd sf : val)
+      pr_content left_content md_content right_content sf_content
+      (kMd kSf : nat) left_triples right_triples,
+      ⌜ d = (pr, ld, md, rd, sf)%V ⌝ ∗
+      ⌜ five_tuple_configuration 3 (length left_content) kMd (length right_content) kSf ⌝ ∗
+      buffer 3 pr_content pr ∗
+      isDeque left_triples ld ∗
+      buffer kMd md_content md ∗
+      isDeque right_triples rd ∗
+      buffer kSf sf_content sf ∗
+      ([∗list] c;tr ∈ left_content;left_triples, ▷ triple c tr) ∗
+      ([∗list] c;tr ∈ right_content;right_triples, ▷ triple c tr) ∗
+      ⌜ o = pr_content ++ List.concat left_content ++ md_content ++ List.concat right_content ++ sf_content ⌝
+  )%I.
+
+  Lemma safe_decidable : forall o f,
+    fiveTuple o f -∗
+      (isUnsafePopFiveTuple o f ∗ WP naive_pop_safe f {{ x, ⌜ x = #false ⌝ }})
+    ∨ isPopFiveTuple o f ∗ WP naive_pop_safe f {{ x, ⌜ x = #true ⌝ }}.
+  Proof.
+    iIntros (o f) "(%p & %l & %m & %r & %s & %op & %ol & %om & %or & %os &
+                      %kPr & %kMd & %kSf & %ltr & %rtr &
+                      %Heq & %conf & #Hp & #Hl & #Hm & #Hr & #Hs &
+                      #Hltr & #Hrtr & %Hoeq)".
+    destruct (dec_eq_nat kPr 3) as [-> | HkPr]; [iLeft | iRight].
+    - iSplitL.
+      + iExists p, l, m, r, s, op, ol, om, or, os, kMd, kSf, ltr, rtr.
+        iFrame "#". iFrame.
+        doneL.
+        iSplit; done.
+      + rewrite /naive_pop_safe Heq.
+        wp_pures.
+        inversion conf.
+        wp_apply (bis_empty_spec with "Hm") as "_".
+        wp_pures.
+        wp_apply (blength_spec with "Hp") as "_".
+        wp_pures.
+        done.
+    - iSplitR.
+      + iExists p, l, m, r, s, op, ol, om, or, os, kPr, kMd, kSf, ltr, rtr.
+        iFrame. iFrame "#".
+        doneL. doneR.
+        iPureIntro.
+        inversion conf.
+        * by easy_config.
+        * inversion H; [ exfalso; lia |].
+          by easy_config.
+      + rewrite /naive_pop_safe Heq.
+        iFrame.
+        wp_pures.
+        wp_apply (bis_empty_spec with "Hm") as "_".
+        inversion conf; wp_pures.
+        * done.
+        * wp_apply (blength_spec with "Hp") as "_".
+          clear H0.
+          invert_all_in; wp_pures; done.
+  Qed.
+
+  Ltac suffix_only_incantation op om H H1 Hoeq :=
+    iDestruct (buffer_length with "Hp") as "%LprC";
+    destruct op; [| inversion LprC];
+    iDestruct (buffer_length with "Hm") as "%LmdC";
+    destruct om; [| inversion LmdC];
+    symmetry in H; rewrite (nil_length_inv _ H) in Hoeq |- *;
+    symmetry in H1; rewrite (nil_length_inv _ H1) in Hoeq |- *;
+    iDestruct (big_sepL2_nil_inv_l with "Hltr") as "->";
+    iDestruct (big_sepL2_nil_inv_l with "Hrtr") as "->".
+
+  Lemma safe_naive_pop : forall o f,
+    {{{ isPopFiveTuple o f }}}
+      naive_pop f
+    {{{ x d o', RET (x, d)%V; isDeque o' d ∗ ⌜ o = ⋅x ++ o' ⌝ }}}.
+  Proof.
+    iIntros (o f ψ) "Hf Hψ".
+    iDestruct "Hf" as "(%p & %l & %m & %r & %s & %op & %ol & %om & %or & %os &
+                      %kPr & %kMd & %kSf & %ltr & %rtr &
+                      -> & %conf & #Hp & #Hl & #Hm & #Hr & #Hs &
+                      #Hltr & #Hrtr & %Hoeq)".
+    rewrite /naive_pop.
+    wp_pures.
+    wp_apply (bis_empty_spec with "Hm") as "_".
+    inversion conf; wp_pures.
+    - suffix_only_incantation op om H H1 Hoeq.
+      change (kSf ∈ map S [0;1;2;3;4;5;6;7]) in H3.
+      assert (∃ kSf', kSf = kSf' + 1) as (kSf' & ->)
+        by (invert_all_in;
+        match goal with
+        | |- ∃ kSf', S ?x = kSf' + 1 => exists x; lia
+        end).
+      wp_apply (bpop_spec with "Hs") as "%b' %x %o' (#Hb & ->)".
+      rewrite /assemble /assemble_.
+      wp_pures.
+      wp_apply (bis_empty_spec with "Hm") as "_". wp_pures.
+      wp_apply (bis_empty_spec with "Hb") as "_".
+      destruct kSf'; wp_pures.
+      + iApply "Hψ".
+        iDestruct (buffer_length with "Hb") as "%LbC".
+        destruct o'; [| inversion LbC].
+        iModIntro.
+        iSplit.
+        * by isEmptyDeque.
+        * iPureIntro.
+          rewrite Hoeq //.
+      + wp_bind (ref _)%E.
+        wp_apply (csref_alloc (fiveTuple o')) as "%ℓ'' #Hℓ''".
+        * iExists p,l,m,r,b',[],[],[],[],o',0,0,(S kSf'),[],[].
+          rewrite /concat !app_nil_l in Hoeq.
+          iFrame. iFrame "#".
+          doneL.
+          assert (S kSf' ∈ [1..7]).
+            { assert (S kSf' + 1 = S (S kSf')) as Heq by lia.
+              rewrite Heq in H3.
+              invert_all_in; list_elem_of.
+            }
+          clear H3.
+          iSplit. iPureIntro. by constructor; invert_all_in; list_elem_of.
+          do 2 doneL.
+          iPureIntro.
+          rewrite //.
+        * wp_pures.
+          iModIntro.
+          iApply "Hψ".
+          iSplit. by ℓisDeque ℓ''.
+          iPureIntro. rewrite Hoeq //.
+    - change (kPr ∈ map S [3;4;5]) in H.
+      apply decrease_in in H as (kP & -> & H).
+      wp_apply (bpop_spec with "Hp") as "%b' %x %o' (#Hb' & ->)".
+      rewrite /assemble_.
+      wp_pures.
+      wp_apply (csref_alloc (fiveTuple _)) as "%ℓ'' #Hℓ''".
+      + iExists b',l,m,r,s,o',ol,om,or,os,kP,kMd,kSf,ltr,rtr.
+        rewrite -H3.
+        iFrame. iFrame "#".
+        doneL.
+        iSplit. iPureIntro. by constructor; invert_all_in; list_elem_of.
+        iSplit. iApply (big_sepL2_mono with "Hltr"). by auto.
+        iSplit. iApply (big_sepL2_mono with "Hrtr"). by auto.
+        done.
+      + wp_pures.
+        iModIntro.
+        iApply "Hψ".
+        iSplit. by ℓisDeque ℓ''.
+        iPureIntro. rewrite Hoeq. aac_reflexivity.
+  Qed.
+
+  Lemma unsafe_naive_pop : forall o f,
+    {{{ fiveTuple o f }}}
+      naive_pop f
+    {{{ x (d : val) o', RET (x, d)%V;
+      ⌜ o = ⋅ x ++ o' ⌝ ∗
+      ∀ y : val,
+        WP push y d {{ d, isDeque (⋅ y ++ o') d }}
+    }}}.
+  Proof.
+    iIntros (o f ψ) "Hf Hψ".
+    iDestruct "Hf" as "(%p & %l & %m & %r & %s & %op & %ol & %om & %or & %os &
+                      %kPr & %kMd & %kSf & %ltr & %rtr &
+                      -> & %conf & #Hp & #Hl & #Hm & #Hr & #Hs &
+                      #Hltr & #Hrtr & %Hoeq)".
+    rewrite /naive_pop.
+    wp_pures.
+    wp_apply (bis_empty_spec with "Hm") as "_".
+    inversion conf; wp_pures.
+    - suffix_only_incantation op om H H1 Hoeq.
+      iClear "Hl Hr".
+      change (kSf ∈ map S [0;1;2;3;4;5;6;7]) in H3.
+      apply decrease_in in H3 as (ks & -> & Hks).
+      wp_apply (bpop_spec with "Hs") as (b' x o') "[#Hb' %Hoeq']".
+      rewrite /assemble.
+      wp_pures.
+      wp_apply (bis_empty_spec with "Hm") as "_".
+      wp_pures.
+      wp_apply (bis_empty_spec with "Hb'") as "_".
+      inversion Hks; wp_pures.
+      + iApply "Hψ".
+        iModIntro.
+        iSplit.
+        * iPureIntro.
+          aac_rewrite Hoeq.
+          rewrite //.
+        * iIntros (y).
+          rewrite /push.
+          wp_pures.
+          iDestruct (TIME_CHEAT _) as "τ".
+          wp_apply (tick_spec with "τ") as "_".
+          rewrite /asingleton.
+          wp_pures.
+          wp_apply (bpush_spec) as (b) "Hb". by iApply bempty_spec.
+          wp_pures.
+          wp_apply (csref_alloc (fiveTuple [y]) with "[Hb]") as (ℓ) "Hℓ".
+            { iExists bempty, NONEV, bempty, NONEV, b, [], [], [], [], [y], 0, 0, 1, [], [].
+              iFrame. iFrame "#".
+              repeat doneL.
+              iSplit. by easy_config.
+              repeat (iSplit; [iApply bempty_spec || isEmptyDeque |]).
+              do 2 doneL.
+              done.
+            }
+          wp_pures.
+          iModIntro.
+          rewrite /=.
+          iDestruct (buffer_length with "Hs") as "%Hos".
+          destruct os; [inversion Hos |].
+          destruct os; [| inversion Hos].
+          destruct o'; [| inversion Hoeq'].
+          ℓisDeque ℓ.
+          iExact "Hℓ".
+      + clear Hks.
+        assert (bool_decide (ks = 0%nat) = false) as -> by invert_all_in.
+        rewrite /assemble_.
+        wp_pures.
+        wp_alloc ℓ as "Hℓ".
+        wp_pures.
+        iModIntro.
+        iApply "Hψ".
+        iSplit. iPureIntro; aac_rewrite Hoeq; by rewrite //.
+        iIntros (y').
+        rewrite /push.
+        wp_pures.
+        iDestruct (TIME_CHEAT _) as "τ".
+        wp_apply (tick_spec with "τ") as "_".
+        wp_pures.
+        wp_load.
+        wp_pures.
+        wp_apply (bis_empty_spec with "Hm") as "_".
+        wp_pures.
+        wp_apply (bhas_length_8_spec with "Hb'") as "_".
+        assert (bool_decide (ks = 8%nat) = false) as -> by invert_all_in.
+        wp_pures.
+        wp_store.
+        rewrite /assemble_.
+        wp_apply (bpush_spec with "Hb'") as (b) "Hb".
+        wp_pures.
+        wp_apply (csref_alloc (fiveTuple (⋅y' ++ o')) with "[Hb]") as (ℓ') "Hℓ'".
+          { iExists bempty, NONEV, bempty, NONEV, b, [], [], [], [], (⋅y' ++ o'), 0, 0, (ks+1), [], [].
+            iFrame. iFrame "#".
+            repeat doneL.
+            iSplit. rewrite H H1 -H0 -H2 in conf. done.
+            repeat (iSplit; [iApply bempty_spec || isEmptyDeque |]).
+            do 2 doneL.
+            done.
+          }
+        wp_pures.
+        iModIntro.
+        rewrite /=.
+        ℓisDeque ℓ'.
+        iExact "Hℓ'".
+    - change (kPr ∈ map S [2; 3; 4; 5]) in H.
+      apply decrease_in in H as (kp & -> & Hkp).
+      wp_apply (bpop_spec with "Hp") as "%b' %x %o' (#Hb' & ->)".
+      rewrite /assemble_.
+      wp_pures.
+      wp_alloc ℓ as "Hℓ".
+      wp_pures.
+      iModIntro.
+      iApply ("Hψ" $! x (SOMEV #ℓ) (o' ++ concat ol ++ om ++ concat or ++ os)).
+      iSplit. iPureIntro. rewrite Hoeq. aac_reflexivity.
+      iIntros (y).
+      rewrite /push.
+      wp_pures.
+      iDestruct (TIME_CHEAT _) as "τ".
+      wp_apply (tick_spec with "τ") as "_".
+      wp_pures.
+      wp_load.
+      wp_pures.
+      wp_apply (bis_empty_spec with "Hm") as "_".
+      wp_pures.
+      wp_apply (bhas_length_6_spec with "Hb'") as "_".
+      assert (bool_decide (kp = 6%nat) = false) as  -> by invert_all_in.
+      wp_pures.
+      wp_store.
+      rewrite /assemble_.
+      wp_apply (bpush_spec with "Hb'") as "%p' #Hp'".
+      wp_pures.
+      wp_apply (csref_alloc (fiveTuple (⋅y ++ o' ++ concat ol ++ om ++ concat or ++ os))) as "%ℓ' Hℓ'".
+      + iExists p',l,m,r,s,(⋅y++o'),ol,om,or,os,(kp+1),2,kSf,ltr,rtr.
+        iFrame "#".
+        doneL.
+        iSplit. iPureIntro. rewrite H3. done.
+        iSplit. iApply (big_sepL2_mono with "Hltr"). by auto.
+        iSplit. iApply (big_sepL2_mono with "Hrtr"). by auto.
+        done.
+      + wp_pures.
+        iModIntro.
+        ℓisDeque ℓ'.
+        iExact "Hℓ'".
+  Qed.
+
+  Lemma inspect_first_spec : forall o f,
+    {{{ fiveTuple o f }}}
+      inspect_first f
+    {{{ o' t, RET t; ⌜ o = ⋅ t ++ o' ⌝  }}}.
+  Proof.
+    iIntros (o f ψ) "Hf Hψ".
+    iDestruct "Hf" as "(%p & %l & %m & %r & %s & %op & %ol & %om & %or & %os &
+                      %kPr & %kMd & %kSf & %ltr & %rtr &
+                      -> & %conf & #Hp & #Hl & #Hm & #Hr & #Hs &
+                      #Hltr & #Hrtr & %Hoeq)".
+    rewrite /inspect_first. wp_pures.
+    wp_apply (bis_empty_spec with "Hm") as "_".
+    inversion conf; wp_pures.
+    - change (kSf ∈ map S [0;1;2;3;4;5;6;7]) in H3.
+      apply decrease_in in H3 as (kS & -> & HkS).
+      destruct os.
+        { iDestruct (buffer_length with "Hs") as "%abs".
+          simpl in abs; lia. }
+      wp_apply (bfirst_spec with "Hs") as "_".
+      iApply "Hψ".
+      suffix_only_incantation op om H H1 Hoeq.
+      iPureIntro.
+      rewrite Hoeq //.
+    - change (kPr ∈ map S [2;3;4;5]) in H.
+      apply decrease_in in H as (kP & -> & HkP).
+      destruct op.
+        { iDestruct (buffer_length with "Hp") as "%abs".
+          simpl in abs; lia. }
+      wp_apply (bfirst_spec with "Hp") as "_".
+      iApply "Hψ".
+      iPureIntro.
+      rewrite Hoeq //.
+  Qed.
+
+  Inductive special_triple_configuration : nat -> nat -> nat -> Prop :=
+    | is_special_three : forall y, y ∈ [0; 2; 3] -> special_triple_configuration 3 0 y
+    | is_special_child : forall x o y, x ∈ [2; 3] -> o > 0 -> y ∈ [2; 3] -> special_triple_configuration x o y
+    | is_special_last : forall x o y, x ∈ [2; 3] -> y ∈ [2; 3] -> special_triple_configuration x o y.
+
+  Inductive not_special_triple_configuration : nat -> nat -> nat -> Prop :=
+    (* | is_bad : forall y, y ∈ [0; 2; 3] -> not_special_triple_configuration 2 0 y. *)
+    | is_bad : not_special_triple_configuration 2 0 0.
+
+  Definition isSpecialTriple := (
+    λ o t,
+      ∃ (fst ch lst : val)
+        fst_content child_content lst_content
+        (kFst kLst : nat) triples,
+        ⌜ special_triple_configuration kFst (length child_content) kLst ⌝ ∗
+        ⌜ t = (fst, ch, lst)%V ⌝ ∗
+        buffer kFst fst_content fst ∗
+        isDeque triples ch ∗
+        buffer kLst lst_content lst ∗
+        ([∗list] c;tr ∈ child_content;triples, ▷ triple c tr) ∗
+        ⌜ o = fst_content ++ List.concat child_content ++ lst_content ⌝
+  )%I.
+
+  Definition isNotSpecialTriple := (
+    λ o t,
+      ∃ (fst ch lst : val)
+        fst_content child_content lst_content
+        (kFst kLst : nat) triples,
+        ⌜ not_special_triple_configuration kFst (length child_content) kLst ⌝ ∗
+        ⌜ t = (fst, ch, lst)%V ⌝ ∗
+        buffer kFst fst_content fst ∗
+        isDeque triples ch ∗
+        buffer kLst lst_content lst ∗
+        ([∗list] c;tr ∈ child_content;triples, ▷ triple c tr) ∗
+        ⌜ o = fst_content ++ List.concat child_content ++ lst_content ⌝
+  )%I.
+
+  Lemma special_decidable : forall o t,
+    triple o t -∗
+      isSpecialTriple o t
+    ∨ isNotSpecialTriple o t.
+  Proof.
+    iIntros (o t) "Ht".
+    rewrite triple_unfold.
+    iDestruct "Ht" as (f c l fc cc lc kFst kLst tr) "(%conf & -> & Hf & Hc & Hl & Htr & %Hoeq)".
+    inversion conf.
+    - inversion H0.
+      + inversion H2.
+        * iRight.
+          iExists f, c, l, fc, cc, lc, kFst, 0, tr.
+          rewrite H6.
+          iFrame.
+          iSplit; [| iSplit]; iPureIntro; auto.
+          rewrite -H. constructor; done.
+        * iLeft.
+          iExists f, c, l, fc, cc, lc, kFst, kLst, tr.
+          rewrite H6.
+          iFrame.
+          iSplit; [| iSplit]; iPureIntro; auto.
+          rewrite -H. apply is_special_last; by list_elem_of.
+      + clear H0. assert (kFst = 3) as H' by (clear H2; invert_all_in).
+        iLeft.
+        iExists f, c, l, fc, cc, lc, kFst, kLst, tr.
+        iFrame.
+        iSplit; [| iSplit]; iPureIntro; auto.
+        rewrite -H H'. constructor; done.
+    - inversion H; [| inversion H]; [| clear H H1; invert_all_in; lia |].
+      + iLeft.
+        iExists f, c, l, fc, cc, lc, kFst, kLst, tr.
+        rewrite H7.
+        iFrame.
+        iSplit; [| iSplit]; iPureIntro; auto.
+        -- constructor; auto; list_elem_of.
+      + iLeft.
+        iExists f, c, l, fc, cc, lc, kFst, kLst, tr.
+        assert (kFst = 3) as -> by (clear H H1; invert_all_in).
+        iFrame.
+        iSplit; [| iSplit]; iPureIntro; auto.
+        constructor; auto.
+  Qed.
+
+  Definition isPersFiveTupleLaterRemoved := (
+    λ o d, ∃ (pr ld md rd sf : val)
+      pr_content left_content md_content right_content sf_content
+      (kPr kMd kSf : nat) left_triples right_triples,
+      ⌜ d = (pr, ld, md, rd, sf)%V ⌝ ∗
+      ⌜ five_tuple_configuration kPr (length left_content) kMd (length right_content) kSf ⌝ ∗
+      buffer kPr pr_content pr ∗
+      isDeque left_triples ld ∗
+      buffer kMd md_content md ∗
+      isDeque right_triples rd ∗
+      buffer kSf sf_content sf ∗
+      ([∗list] c;tr ∈ left_content;left_triples, triple c tr) ∗
+      ([∗list] c;tr ∈ right_content;right_triples, triple c tr) ∗
+      ⌜ o = pr_content ++ List.concat left_content ++ md_content ++ List.concat right_content ++ sf_content ⌝
+  )%I.
+
+  Lemma add_later : forall o d, isPersFiveTupleLaterRemoved o d -∗ fiveTuple o d.
+  Proof.
+    iIntros (o d) "Hd".
+    iDestruct "Hd" as (p l m r s op ol om or os kp km ks ltr rtr)
+      "(-> & conf & hp & hl & hm & hr & hs & hltr & hrtr & heq)".
+    iExists p, l, m, r, s, op, ol, om, or, os, kp, km, ks, ltr, rtr.
+    iFrame.
+    doneL.
+    iSplitL "hltr".
+    - iApply (big_sepL2_mono with "hltr"). by auto.
+    - iApply (big_sepL2_mono with "hrtr"). by auto.
+  Qed.
+
+  Lemma pop_triple_spec : forall os tr ℓ,
+    {{{ ℓ ⤇ fiveTuple tr
+      ∗ ([∗list] x;y ∈ os;tr, triple x y)
+      ∗ (∀ ℓ x o,
+          ℓ ⤇ fiveTuple (⋅ x ++ o) -∗
+          WP pop_nonempty #ℓ
+            {{ r, ∃ d, ⌜ r = (x, d)%V ⌝ ∗ isDeque o d }})
+    }}}
+      subst "pop_nonempty" pop_nonempty (pop_triple #ℓ)
+    {{{ t o tr' os' (d' : val), RET (t, d')%V;
+      ⌜ tr = ⋅t ++ tr' ∧ os = ⋅o ++ os' ⌝ ∗
+      ([∗list] x;y ∈ os';tr', triple x y) ∗
+      ( isSpecialTriple o t ∗ (∀ x : val, WP push x d' {{ d'', isDeque (⋅x ++ tr') d'' }})
+      ∨ isNotSpecialTriple o t ∗ isDeque tr' d'
+      )
+    }}}.
+  Proof.
+    iIntros (os tr d Hψ) "(#Hd & Htr & iH) Hψ".
+    rewrite /pop_triple.
+    wp_pures.
+    wp_apply (csref_load with "Hd").
+    iIntros (f) "#Hf".
+    wp_pures.
+    wp_apply (inspect_first_spec with "[Hf]").
+      { iApply add_later.
+        iExact "Hf".
+      }
+    iIntros (o t) "->".
+    wp_pures.
+    destruct os. iDestruct (big_sepL2_nil_inv_l with "Htr") as "%No". inversion No.
+    assert (l :: os = ⋅ l ++ os) as -> by auto.
+    iDestruct (big_sepL2_app_inv with "Htr") as "(Ht & Htr)". by left.
+    iAssert (triple l t) with "[Ht]" as "Ht".
+      { simpl. iDestruct "Ht" as "[A _]". done. }
+    iDestruct (special_decidable with "Ht") as "[#Ht' | #Ht']";
+    iCombine "Ht' Ht'" as "[Ht! Ht!']";
+    iDestruct "Ht!'" as (fi c la fc cc lc kF kL tr) "(%conf & -> & Hf' & Hc & Hl & Htrtr & %Hleq)";
+    inversion conf.
+    Opaque isSpecialTriple isNotSpecialTriple.
+    + rewrite isDeque_unfold.
+      iDestruct "Hc" as "[[-> ->] | (%ℓ & -> & Hℓ)]".
+      2: {
+        wp_bind (Fst _)%V.
+        iInv "Hℓ" as "(%v' & Hv' & Hℓ')".
+        wp_pure.
+        iExFalso.
+        iDestruct "Hv'" as (pr' ld' md' rd' sf' pc' lc' mc' rc' sc' kp' km' ks' lt rt) "(_ & %conf' & _ & _ & _ & _ & Hs & _ & _ & ->)".
+        iDestruct (big_sepL2_length with "Htrtr") as "%Hlen".
+        rewrite Hlen in H.
+        iDestruct (buffer_length with "Hs") as "%Hslen".
+        assert (ks' > 0) as Hslen' by (inversion conf'; invert_all_in; lia).
+        rewrite !length_app in H.
+        lia.
+      }
+      wp_pures.
+      wp_apply (bhas_length_3_spec with "Hf'") as "_".
+      wp_pures.
+      wp_apply (unsafe_naive_pop).
+        { iFrame.
+          iApply add_later.
+          by iExact "Hf". }
+      iIntros (x d' o') "(%Hoeq' & Hpush)".
+      inversion Hoeq'.
+      iApply "Hψ".
+      doneL.
+      iSplit. iExact "Htr".
+      iLeft.
+      iSplitR.
+      * assert (x = (fi, NONEV, la)%V) as -> by by inversion Hoeq'.
+        iExact "Ht!".
+      * iExact "Hpush".
+    + (* NOTE(Juliette): dedup *)
+      wp_pures.
+      rewrite isDeque_unfold.
+      iDestruct "Hc" as "[[-> ->] | (%ℓ & -> & Hℓ)]".
+        { iDestruct (big_sepL2_nil_inv_r with "Htrtr") as "->". inversion H0. }
+      wp_pures.
+      wp_apply (bhas_length_3_spec with "Hf'") as "_".
+      assert (kF = 2 ∨ kF = 3) as [-> | ->] by invert_all_in; wp_pures.
+      * wp_apply (bis_empty_spec with "Hl") as "_".
+        assert (bool_decide (kL = 0%nat) = false) as -> by invert_all_in.
+        wp_pures.
+        wp_apply (unsafe_naive_pop).
+          { iFrame.
+            iApply add_later.
+            iExact "Hf". }
+        iIntros (x' d' o') "(%Hoeq' & Hpush)".
+        inversion Hoeq'.
+        iApply "Hψ".
+        iFrame.
+        doneL.
+        iLeft.
+        iSplitR.
+        -- assert (x' = (fi, SOMEV #ℓ, la)%V) as -> by by inversion Hoeq'.
+          iExact "Ht!".
+        -- iExact "Hpush".
+      * wp_apply (unsafe_naive_pop).
+          { iFrame.
+            iApply add_later.
+            by iExact "Hf". }
+        iIntros (x' d' o') "(%Hoeq' & Hpush)".
+        inversion Hoeq'.
+        iApply "Hψ".
+        iFrame.
+        doneL.
+        iLeft.
+        iSplitR.
+        -- assert (x' = (fi, SOMEV #ℓ, la)%V) as -> by by inversion Hoeq'.
+          iExact "Ht!".
+        -- iExact "Hpush".
+    + wp_pures.
+      rewrite isDeque_unfold.
+      wp_pures.
+      wp_apply (bhas_length_3_spec with "Hf'") as "_".
+      wp_pures.
+      assert (kF = 2 ∨ kF = 3) as [-> | ->] by invert_all_in; wp_pures.
+      * wp_apply (bis_empty_spec with "Hl") as "_".
+        wp_pures.
+        assert (bool_decide (kL = 0%nat) = false) as -> by invert_all_in.
+        wp_pures.
+        wp_apply (unsafe_naive_pop).
+          { iFrame.
+            iApply add_later.
+            iExact "Hf". }
+        iIntros (x' d' o') "(%Hoeq' & Hpush)".
+        inversion Hoeq'.
+        iApply "Hψ".
+        iFrame.
+        doneL.
+        iLeft.
+        iSplitR.
+        -- assert (x' = (fi, c, la)%V) as -> by by inversion Hoeq'.
+          iExact "Ht!".
+        -- iExact "Hpush".
+      * wp_apply (unsafe_naive_pop).
+          { iApply add_later.
+            by iExact "Hf". }
+        iIntros (x' d' o') "(%Hoeq' & Hpush)".
+        inversion Hoeq'.
+        iApply "Hψ".
+        iFrame.
+        doneL.
+        iLeft.
+        iSplitR.
+        -- assert (x' = (fi, c, la)%V) as -> by by inversion Hoeq'.
+          iExact "Ht!".
+        -- iExact "Hpush".
+    + wp_pures.
+      wp_apply (bhas_length_3_spec with "Hf'") as "_".
+      wp_pures.
+      wp_apply (bis_empty_spec with "Hl") as "_".
+      wp_pures.
+      iApply (wp_strong_mono with "[iH]").
+        { auto. } { reflexivity. }
+      * iApply ("iH"). iExact "Hd".
+      * iIntros (v) "(%d' & -> & Hd')".
+        iApply "Hψ".
+        iModIntro. iFrame. doneL.
+        iRight.
+        iFrame. iExact "Ht!".
+  Qed.
+
+  Lemma prepare_pop_spec : forall o f,
+    {{{ isUnsafePopFiveTuple o f ∗
+      ∀ ℓ x o', ℓ ⤇ fiveTuple (⋅x ++ o') -∗
+        WP pop_nonempty #ℓ {{ r, ∃ d, ⌜ r = (x, d)%V ⌝ ∗ isDeque o' d }}
+    }}}
+      subst "pop_nonempty" pop_nonempty (prepare_pop f)
+    {{{ f', RET f'; isPopFiveTuple o f' }}}.
+  Proof.
+    iIntros (o f ψ) "(Hf & iH) Hψ".
+    rewrite /isUnsafePopFiveTuple.
+    iDestruct "Hf" as "(%p & %l & %m & %r & %s & %op & %ol & %om & %or & %os &
+                      %kMd & %kSf & %ltr & %rtr &
+                      -> & %conf & #Hp & #Hl & #Hm & #Hr & #Hs &
+                      #Hltr & #Hrtr & %Hoeq)".
+    rewrite /prepare_pop.
+    wp_pures.
+    inversion conf.
+    rewrite isDeque_unfold.
+    Notation selpat := "[[-> ->] | (%ℓ & -> & Hℓ)]".
+    iDestruct "Hl" as selpat;
+    [rewrite isDeque_unfold; iDestruct "Hr" as selpat |].
+    - wp_pures.
+      wp_apply (bhas_length_3_spec with "Hs") as "_".
+      iDestruct (big_sepL2_nil_inv_r with "Hltr") as "->";
+      iDestruct (big_sepL2_nil_inv_r with "Hrtr") as "->".
+      inversion H0; wp_pures.
+      + wp_apply (bconcat323_spec with "[Hp Hm Hs]") as "%b' Hb8". by iFrame "#".
+        wp_pures.
+        iApply "Hψ".
+        iModIntro.
+        * iExists bempty, NONEV, bempty, NONEV, b', [], [], [], [], (op++om++os),
+            0, 0, 8, [], [].
+          iFrame. iFrame "#".
+          doneL.
+          iSplit. simpl. iPureIntro. constructor. invert_all_in; list_elem_of.
+          iSplit. by (iApply bempty_spec).
+          iSplit. by isEmptyDeque.
+          iSplit. by (iApply bempty_spec).
+          iSplit. by isEmptyDeque.
+          repeat doneL.
+          iPureIntro.
+          aac_rewrite Hoeq.
+          by rewrite //.
+      + assert (bool_decide (kSf = 3%nat) = false) as ->.
+        { clear H H0. invert_all_in. }
+        wp_pures.
+        change (kSf ∈ map S [3;4;5]) in H8.
+        apply decrease_in in H8 as (k & -> & Hk).
+        clear H0.
+        wp_apply (bdouble_move_left_spec with "[Hp Hm Hs]"). by iFrame "#".
+        iIntros (b1 b2 b3 o1 o2 o3) "(#H1 & #H2 & #H3 & %Heq)".
+        wp_pures.
+        iModIntro.
+        iApply "Hψ".
+        iExists b1, NONEV, b2, NONEV, b3, o1, [], o2, [], o3,
+          4, 2, k, [], [].
+        iFrame. iFrame "#".
+        doneL.
+        iSplit. iPureIntro. constructor; invert_all_in; list_elem_of.
+        iSplit. by isEmptyDeque.
+        iSplit. by isEmptyDeque.
+        repeat doneL.
+        iPureIntro.
+        aac_rewrite Hoeq.
+        rewrite //.
+    - wp_pures.
+      iDestruct (big_sepL2_nil_inv_r with "Hltr") as "->".
+      wp_bind (let: "f" := _ in _)%E.
+      wp_apply (pop_triple_spec with "[iH]").
+      + iSplit. iExact "Hℓ".
+        iSplit. iExact "Hrtr".
+        iApply "iH".
+      + Transparent isSpecialTriple.
+        iIntros (t o' rtr' os' d') "([-> ->] & Htr' & [(#Ht & Hd') | (Ht & Hd')])".
+          (* appeler la spec de pop_case_2_special *)
+        * rewrite /prepare_pop_case_2.
+          iDestruct "Ht" as (fi c la fc cc lc kF kL tr) "(%tconf & -> & #Hfi & #Hc & #Hla & #Htrtr & %Hleq)".
+          wp_pures.
+          wp_apply (bhas_length_3_spec with "Hfi") as "_".
+          inversion tconf; wp_pures.
+          -- wp_apply (bdouble_move_left_spec) as (b1 b2 b3 o1 o2 o3) "(#H1 & #H2 & #H3 & %Hoeq')".
+            { assert (3 = 2 + 1) as -> by reflexivity.
+              iFrame "#". }
+            rewrite /atriple_.
+            wp_pures.
+            wp_bind (push _ _)%E.
+            iApply (wp_strong_mono with "Hd'"). { auto. } { auto. }
+            iIntros (r') "Hr'".
+            iModIntro. wp_pures.
+            iModIntro.
+            iApply "Hψ".
+            iExists b1, NONEV, b2, r', s, o1, [], o2,
+              (⋅(o3 ++ List.concat cc ++ lc) ++ os'), os, 4, 2, kSf,
+              [], (⋅(b3, c, la)%V ++ rtr').
+            doneL.
+            iFrame "#". iFrame.
+            iSplit. iPureIntro. by easy_config.
+            iSplit. by isEmptyDeque.
+            doneL.
+            iSplit; [ iApply (big_sepL2_app) |].
+            ++ simpl; doneR.
+              iNext. iClear "Hrtr".
+              rewrite triple_unfold.
+              iExists b3, c, la, o3, cc, lc, 2, kL, tr.
+              iSplit. iPureIntro. rewrite -H6. by easy_config.
+              doneL. iFrame "#".
+              iSplit. iApply (big_sepL2_mono with "Htrtr"). by auto.
+              iPureIntro.
+              done.
+            ++ iDestruct (big_sepL2_app_inv with "Hrtr") as "[_ Hrtr']". by left.
+              iApply (big_sepL2_mono with "Hrtr'"). by auto.
+            ++ iPureIntro.
+              rewrite Hoeq /= -!app_assoc Hleq.
+              aac_rewrite Hoeq'.
+              aac_reflexivity.
+          -- assert (kF = 2 ∨ kF = 3) as HkF by (clear H H0 H8; invert_all_in).
+            destruct HkF as [-> | ->]; wp_pures.
+            ++ wp_apply (bconcat32_spec with "[Hp Hm]") as (b') "Hb'". by iFrame "#".
+              wp_pures.
+              rewrite isDeque_unfold.
+              iDestruct "Hc" as "[[_ ->] | (%ℓc & -> & Hℓc)]".
+                { iDestruct (big_sepL2_nil_inv_r with "Htrtr") as "->". inversion H7. }
+              wp_pures.
+              wp_apply (abuffer_spec_explicit with "Hla") as "Ht". by assumption.
+              wp_pures.
+              wp_bind (push _ _)%E.
+              iApply (wp_strong_mono with "Hd'"). { auto. } { auto. }
+              iIntros (r') "Hr'".
+              iModIntro. wp_pures.
+              wp_apply (dconcat_spec_helper with "[Hℓc Hr']") as (r) "Hr".
+                { iFrame. ℓisDeque ℓc. iExact "Hℓc". }
+              wp_pures.
+              iModIntro.
+              iApply "Hψ".
+              iExists b', NONEV, fi, r, s, (op++om), [], fc, (cc++⋅lc++os'), os,
+                5, 2, kSf, [], (tr++⋅(la, NONEV, bempty)%V++rtr').
+              doneL.
+              iSplit. iPureIntro. by easy_config.
+              iFrame. iFrame "#".
+              iSplit. by isEmptyDeque.
+              doneL.
+              iSplit.
+              ** iSplit. iApply (big_sepL2_mono with "Htrtr"). by auto.
+                doneL.
+                iApply (big_sepL2_mono with "Htr'"). by auto.
+              ** iPureIntro.
+                rewrite !concat_app Hoeq Hleq /= !app_nil_r.
+                aac_reflexivity.
+            ++ wp_apply (bdouble_move_left_spec with "[Hp Hm Hfi]").
+                { iFrame "#". assert (3 = 2 + 1) as -> by reflexivity. done. }
+             iIntros (b1 b2 b3 o1 o2 o3) "(H1 & H2 & #H3 & %Hnoeq)".
+              rewrite /atriple_.
+              wp_pures.
+              wp_bind (push _ _)%E.
+              iApply (wp_strong_mono with "Hd'"). { auto. } { auto. }
+              iIntros (r') "Hr'".
+              iModIntro.
+              wp_pures.
+              iModIntro. iApply "Hψ".
+              iExists b1, NONEV, b2, r', s, o1, [], o2, (⋅(o3++List.concat cc++lc) ++ os'), os,
+                4, 2, kSf, [], (⋅(b3, c, la)%V ++ rtr').
+              doneL.
+              iSplit. iPureIntro. simpl. by easy_config.
+              iFrame "#". iFrame.
+              iSplit. by isEmptyDeque.
+              doneL.
+              iSplit; [ iApply (big_sepL2_app) |].
+              ** simpl. doneR. iNext.
+                rewrite !triple_unfold.
+                iExists b3, c, la, o3, cc, lc, 2, kL, tr.
+                iSplit. iPureIntro. by easy_config.
+                doneL.
+                iFrame . iFrame "#".
+                iSplit. iApply (big_sepL2_mono with "Htrtr"). by auto.
+                done.
+              ** iApply (big_sepL2_mono with "Htr'"). by auto.
+              ** iPureIntro.
+                rewrite !concat_app Hoeq Hleq /= !app_nil_r.
+                aac_rewrite Hnoeq.
+                aac_reflexivity.
+          -- assert (kF = 2 ∨ kF = 3) as HkF by (clear H H0 H8; invert_all_in).
+            destruct HkF as [-> | ->]; wp_pures.
+            ++ wp_apply (bconcat32_spec with "[Hp Hm]") as (b') "Hb'". by iFrame "#".
+              wp_pures.
+              destruct (bool_decide (c = NONEV)); wp_pures.
+              ** wp_apply (bis_empty_spec with "Hla") as "_".
+                assert (bool_decide (kL = 0%nat) = false) as -> by invert_all_in.
+                wp_pures.
+                wp_apply (abuffer_spec_explicit with "Hla") as "Ht". by assumption.
+                wp_pures.
+                wp_bind (push _ _)%E.
+                iApply (wp_strong_mono with "Hd'"). { auto. } { auto. }
+                iIntros (r') "Hr'".
+                iModIntro. wp_pures.
+                wp_apply (dconcat_spec_helper with "[Hc Hr']") as (r) "Hr".
+                  { iFrame. by iFrame "#". }
+                wp_pures.
+                iModIntro.
+                iApply "Hψ".
+                iExists b', NONEV, fi, r, s, (op++om), [], fc, (cc++⋅lc++os'), os,
+                  5, 2, kSf, [], (tr++⋅(la, NONEV, bempty)%V++rtr').
+                doneL.
+                iSplit. iPureIntro. by easy_config.
+                iFrame. iFrame "#".
+                iSplit. by isEmptyDeque.
+                doneL.
+                iSplit.
+                --- iSplit. iApply (big_sepL2_mono with "Htrtr"). by auto.
+                  doneL.
+                  iApply (big_sepL2_mono with "Htr'"). by auto.
+                --- iPureIntro.
+                  rewrite !concat_app Hoeq Hleq /= !app_nil_r.
+                  aac_reflexivity.
+              ** wp_apply (abuffer_spec_explicit with "Hla") as "Ht". by assumption.
+                wp_pures.
+                wp_bind (push _ _)%E.
+                iApply (wp_strong_mono with "Hd'"). { auto. } { auto. }
+                iIntros (r') "Hr'".
+                iModIntro. wp_pures.
+                wp_apply (dconcat_spec_helper with "[Hc Hr']") as (r) "Hr".
+                  { iFrame. by iFrame "#". }
+                wp_pures.
+                iModIntro.
+                iApply "Hψ".
+                iExists b', NONEV, fi, r, s, (op++om), [], fc, (cc++⋅lc++os'), os,
+                  5, 2, kSf, [], (tr++⋅(la, NONEV, bempty)%V++rtr').
+                doneL.
+                iSplit. iPureIntro. by easy_config.
+                iFrame. iFrame "#".
+                iSplit. by isEmptyDeque.
+                doneL.
+                iSplit.
+                --- iSplit. iApply (big_sepL2_mono with "Htrtr"). by auto.
+                  doneL.
+                  iApply (big_sepL2_mono with "Htr'"). by auto.
+                --- iPureIntro.
+                  rewrite !concat_app Hoeq Hleq /= !app_nil_r.
+                  aac_reflexivity.
+            ++ wp_apply (bdouble_move_left_spec) as (b1 b2 b3 o1 o2 o3) "(#H1 & #H2 & #H3 & %Hoeq')".
+            { assert (3 = 2 + 1) as -> by reflexivity.
+              iFrame "#". }
+            rewrite /atriple_.
+            wp_pures.
+            wp_bind (push _ _)%E.
+            iApply (wp_strong_mono with "Hd'"). { auto. } { auto. }
+            iIntros (r') "Hr'".
+            iModIntro. wp_pures.
+            iModIntro.
+            iApply "Hψ".
+            iExists b1, NONEV, b2, r', s, o1, [], o2,
+              (⋅(o3 ++ List.concat cc ++ lc) ++ os'), os,
+              4, 2, kSf,
+              [], (⋅(b3, c, la)%V ++ rtr').
+            doneL.
+            iSplit. iPureIntro. by easy_config.
+            iFrame. iFrame "#".
+            iSplit. by isEmptyDeque.
+            doneL.
+            iSplit; [ iApply (big_sepL2_app) |].
+            ** simpl; doneR.
+              iNext. iClear "Hrtr".
+              rewrite triple_unfold.
+              iExists b3, c, la, o3, cc, lc, 2, kL, tr.
+              iSplit. iPureIntro. destruct (length cc); constructor; clear H H0; invert_all_in; by (list_elem_of || auto with arith).
+              doneL. iFrame "#".
+              iSplit. iApply (big_sepL2_mono with "Htrtr"). by auto.
+              iPureIntro.
+              done.
+            ** iDestruct (big_sepL2_app_inv with "Hrtr") as "[_ Hrtr']". by left.
+              iApply (big_sepL2_mono with "Hrtr'"). by auto.
+            ** iPureIntro.
+              rewrite Hoeq /= -!app_assoc Hleq.
+              aac_rewrite Hoeq'.
+              aac_reflexivity.
+        Opaque isSpecialTriple.
+        * Transparent isNotSpecialTriple. wp_pures.
+          (* appeler la spec de pop_case_2_not_special *)
+          rewrite /prepare_pop_case_2.
+          iDestruct "Ht" as (fi c la fc cc lc kF kL tr) "(%tconf & -> & #Hfi & #Hc & #Hla & #Htrtr & %Hleq)".
+          wp_pures.
+          wp_apply (bhas_length_3_spec with "Hfi") as "_".
+          inversion tconf; wp_pures.
+          wp_apply (bconcat32_spec with "[Hp Hm]") as (b') "Hb'". by iFrame "#".
+          rewrite isDeque_unfold.
+          iDestruct "Hc" as "[[-> ->] | (%ℓ' & -> & Hℓ')]".
+          2: {
+            rewrite /abuffer.
+            do 4 wp_pure.
+            wp_bind (_ = _)%E.
+            iInv "Hℓ'" as "(%v' & Hv' & Hℓ'')".
+            wp_pure.
+            iExFalso.
+            iDestruct "Hv'" as (pr' ld' md' rd' sf' pc' lc' mc' rc' sc' kp' km' ks' lt rt) "(_ & %conf' & _ & _ & _ & _ & Hs' & _ & _ & ->)".
+            iDestruct (big_sepL2_length with "Htrtr") as "%Hlen".
+            rewrite Hlen in H8.
+            iDestruct (buffer_length with "Hs'") as "%Hslen".
+            assert (ks' > 0) as Hslen' by (inversion conf'; invert_all_in; lia).
+            rewrite !length_app in H8.
+            lia.
+          }
+          wp_pures.
+          wp_apply (bis_empty_spec with "Hla") as "_".
+          wp_pures.
+          (*
+          assert (kL = 0 ∨ kL ∈ [2; 3]) as Hkl. by invert_all_in.
+          destruct Hkl as [-> | Hkl]; wp_pures.
+          -- *)
+            iModIntro. iApply "Hψ".
+            iExists b', NONEV, fi, d', s, (op ++ om), [], fc, os', os,
+              5, 2, kSf, [], rtr'.
+            doneL.
+            iSplit. iPureIntro. by easy_config.
+            iFrame "#". iFrame.
+            iSplit. by isEmptyDeque.
+            doneL.
+            iSplit. iApply (big_sepL2_mono with "Htr'"). by auto.
+            destruct lc; [| iDestruct (buffer_length with "Hla") as "%No"; by inversion No ].
+            destruct cc; [| by inversion H6 ].
+            iPureIntro.
+            rewrite Hoeq Hleq /= app_nil_r.
+            aac_reflexivity.
+          (*
+          -- assert (bool_decide (kL = 0%nat) = false) as -> by invert_all_in.
+            wp_pures.
+            wp_apply (abuffer_spec_explicit with "Hla") as "Ht". by assumption.
+            wp_pures.
+            wp_bind (push _ _)%E.
+            iApply (wp_strong_mono with "Hd'"). { auto. } { auto. }
+            iIntros (r') "Hr'".
+            iModIntro. wp_pures.
+            iDestruct (split_time time_for_concat with "τ") as "[ι τ]". by lia.
+            wp_apply (dconcat_spec_helper with "[Hℓc Hr' ι O]") as (r) "[Hr O]".
+              { iFrame. ℓisDeque ℓc. iExact "Hℓc". }
+            wp_pures.
+            iModIntro.
+            iApply "Hψ".
+            iSplitR "O"; [| done].
+            iExists b', NONEV, fi, r, s, (op++om), [], fc, (cc++⋅lc++os'), os,
+              5, 2, kSf, [], (tr++⋅(la, NONEV, bempty)%V++rtr').
+            doneL.
+            iSplit. iPureIntro. by easy_config.
+            iSplitL "pot". iDestruct (split_time (5 ⋄ kSf) with "pot") as "[ι _]".
+              clear H H6 H8; invert_all_in; simpl; lia.
+              by iExact "ι".
+            iFrame. iFrame "#".
+            iSplit. by isEmptyDeque.
+            doneL.
+            iSplit.
+            ** iSplit. iApply (big_sepL2_mono with "Htrtr"). by auto.
+              doneL.
+              iApply (big_sepL2_mono with "Htr'"). by auto.
+            ** iPureIntro.
+              rewrite !concat_app Hoeq Hleq /= !app_nil_r.
+              aac_reflexivity.
+      *)
+        Opaque isNotSpecialTriple.
+    - wp_pures.
+      wp_bind (let: "f" := _ in _)%E.
+      wp_apply (pop_triple_spec with "[iH]").
+      + iSplit. iExact "Hℓ".
+        iSplit. iExact "Hltr".
+        iApply "iH".
+      + Transparent isSpecialTriple.
+        iIntros (t o' ltr' os' d') "([-> ->] & Htr' & [(#Ht & Hd') | (Ht & Hd')])".
+        * (* appeler la spec de pop_case_1_special *)
+          rewrite /prepare_pop_case_1.
+          iDestruct "Ht" as (fi c la fc cc lc kF kL tr) "(%tconf & -> & #Hfi & #Hc & #Hla & #Htrtr & %Hleq)".
+          wp_pures.
+          wp_apply (bhas_length_3_spec with "Hfi") as "_".
+          inversion tconf; wp_pures.
+          -- wp_apply (bmove_left_1_33_spec with "[Hp Hfi]"). by iFrame "#".
+            iIntros (b1 b2 o1 o2) "(#H1 & #H2 & %Honeq)".
+            rewrite /atriple_.
+            wp_pures.
+            wp_bind (push _ _)%E.
+            iApply (wp_strong_mono with "Hd'"). { auto. } { auto. }
+            iIntros (l') "Hl'".
+            iModIntro. wp_pures.
+            iModIntro. iApply "Hψ".
+            iExists b1, l', m, r, s, o1, (⋅(o2++List.concat cc++lc) ++ os'), om, or, os,
+              4, 2, kSf, (⋅(b2, c, la)%V ++ ltr'), rtr.
+            doneL.
+            iSplit. iPureIntro. by easy_config.
+            iFrame. iFrame "#".
+            iSplit; [iApply big_sepL2_app; [simpl| ] | iSplit].
+            ++ doneR. iNext.
+              iClear "Hltr".
+              rewrite triple_unfold.
+              iExists b2, c, la, o2, cc, lc, 2, kL, tr.
+              iSplit. iPureIntro. inversion H6. by easy_config.
+              doneL.
+              iFrame "#".
+              iSplit. iApply (big_sepL2_mono with "Htrtr"). by auto.
+              done.
+            ++ iApply (big_sepL2_mono with "Htr'"). by auto.
+            ++ iApply (big_sepL2_mono with "Hrtr"). by auto.
+            ++ iPureIntro.
+              rewrite Hoeq /= -!app_assoc Hleq.
+              aac_rewrite Honeq.
+              aac_reflexivity.
+          -- assert (kF = 2 ∨ kF = 3) as [-> | ->] by invert_all_in; wp_pures.
+            ++ wp_apply (bconcat32_spec with "[Hp Hfi]") as (b') "Hb'". by iFrame "#".
+              wp_pures.
+              rewrite !isDeque_unfold.
+              iDestruct "Hc" as "[[-> ->] | (%ℓc & -> & Hℓc)]".
+                { iDestruct (big_sepL2_nil_inv_r with "Htrtr") as "->". inversion H7. }
+              wp_pures.
+              wp_apply (abuffer_spec_explicit with "Hla") as "Ht". by assumption.
+              wp_pures.
+              wp_bind (push _ _)%E.
+              iApply (wp_strong_mono with "Hd'"). { auto. } { auto. }
+              iIntros (l') "Hl'".
+              iModIntro. wp_pures.
+              wp_apply (dconcat_spec_helper with "[Hℓc Hl']") as (l) "Hl".
+                { iFrame. ℓisDeque ℓc. iExact "Hℓc". }
+              wp_pures.
+              iModIntro.
+              iApply "Hψ".
+              iExists b', l, m, r, s, (op ++ fc), (cc ++ ⋅lc ++ os'), om, or, os,
+                5, 2, kSf, (tr ++ ⋅(la, NONEV, bempty)%V ++ ltr'), rtr.
+              doneL.
+              iSplit. iPureIntro. simpl. by easy_config.
+              rewrite -isDeque_unfold.
+              iFrame "#". iFrame.
+              iSplit; [iSplit; [| iSplit; [done |]] | iSplit].
+              ** iApply (big_sepL2_mono with "Htrtr"). by auto.
+              ** iApply (big_sepL2_mono with "Htr'"). by auto.
+              ** iApply (big_sepL2_mono with "Hrtr"). by auto.
+              ** iPureIntro.
+                rewrite Hoeq Hleq !concat_app {1 6}/concat.
+                aac_reflexivity.
+            ++ wp_apply (bmove_left_1_33_spec with "[Hp Hfi]"). by iFrame "#".
+              iIntros (b1 b2 o1 o2) "(#H1 & #H2 & %Hnoeq)".
+              rewrite /atriple_.
+              wp_pures.
+              wp_bind (push _ _)%E.
+              iApply (wp_strong_mono with "Hd'"). { auto. } { auto. }
+              iIntros (l') "Hl'".
+              iModIntro. wp_pures.
+              iApply "Hψ".
+              iModIntro.
+              iExists b1, l', m, r, s, o1, (⋅(o2++List.concat cc++lc)++os'), om, or, os,
+                4, 2, kSf, (⋅(b2, c, la)%V++ltr'), rtr.
+              doneL.
+              iSplit. iPureIntro. simpl. by easy_config.
+              iFrame "#". iFrame.
+              iSplit; [iApply big_sepL2_app; [simpl |]| iSplit].
+              ** doneR. iNext.
+                iClear "Hltr".
+                rewrite triple_unfold.
+                iExists b2, c, la, o2, cc, lc, 2, kL, tr.
+                iSplitL. iPureIntro. destruct (length cc); [inversion H7 |]; by easy_config.
+                doneL.
+                iFrame "#".
+                iSplit. iApply (big_sepL2_mono with "Htrtr"). by auto.
+                done.
+              ** iApply (big_sepL2_mono with "Htr'"). by auto.
+              ** iApply (big_sepL2_mono with "Hrtr"). by auto.
+              ** iPureIntro.
+                rewrite Hoeq Hleq !concat_app /=.
+                aac_rewrite Hnoeq.
+                aac_reflexivity.
+          -- assert (kF = 2 ∨ kF = 3) as [-> | ->] by invert_all_in; wp_pures.
+            ++ wp_apply (bconcat32_spec with "[Hp Hfi]") as (b') "Hb'". by iFrame "#".
+              wp_pures.
+              wp_bind (if: _ then _ else #false)%E.
+              iApply (wp_strong_mono _ _ _ _ _ (λ v, ⌜ v = #false ⌝)%I). { auto. } { auto. }
+                { destruct (bool_decide (c = NONEV)); wp_pures.
+                - wp_apply (bis_empty_spec with "Hla") as "_".
+                  assert (bool_decide (kL = 0%nat) = false) as -> by invert_all_in.
+                  done.
+                - done.
+                }
+              iIntros (v) "->". iModIntro. wp_pures.
+              wp_apply (abuffer_spec_explicit with "Hla") as "Ht". by assumption.
+              wp_pures.
+              wp_bind (push _ _)%E.
+              iApply (wp_strong_mono with "Hd'"). { auto. } { auto. }
+              iIntros (l') "Hl'".
+              iModIntro. wp_pures.
+              wp_apply (dconcat_spec_helper with "[Hc Hl']") as (l) "Hl".
+                { iFrame. iExact "Hc". }
+              wp_pures.
+              iModIntro.
+              iApply "Hψ".
+              iExists b', l, m, r, s, (op ++ fc), (cc ++ ⋅lc ++ os'), om, or, os,
+                5, 2, kSf, (tr ++ ⋅(la, NONEV, bempty)%V ++ ltr'), rtr.
+              doneL.
+              iSplit. iPureIntro. simpl. by easy_config.
+              iFrame "#". iFrame.
+              iSplit; [iSplit; [| iSplit; [done |]] | iSplit].
+              ** iApply (big_sepL2_mono with "Htrtr"). by auto.
+              ** iApply (big_sepL2_mono with "Htr'"). by auto.
+              ** iApply (big_sepL2_mono with "Hrtr"). by auto.
+              ** iPureIntro.
+                rewrite Hoeq Hleq !concat_app {1 6}/concat.
+                aac_reflexivity.
+            ++ wp_apply (bmove_left_1_33_spec with "[Hp Hfi]"). by iFrame "#".
+              iIntros (b1 b2 o1 o2) "(#H1 & #H2 & %Hnoeq)".
+              rewrite /atriple_.
+              wp_pures.
+              wp_bind (push _ _)%E.
+              iApply (wp_strong_mono with "Hd'"). { auto. } { auto. }
+              iIntros (l') "Hl'".
+              iModIntro. wp_pures.
+              iApply "Hψ".
+              iModIntro.
+              iExists b1, l', m, r, s, o1, (⋅(o2++List.concat cc++lc)++os'), om, or, os,
+                4, 2, kSf, (⋅(b2, c, la)%V++ltr'), rtr.
+              doneL.
+              iSplit. iPureIntro. simpl. by easy_config.
+              iFrame "#". iFrame.
+              iSplit; [iApply big_sepL2_app; [simpl |]| iSplit].
+              ** doneR. iNext.
+                iClear "Hltr".
+                rewrite triple_unfold.
+                iExists b2, c, la, o2, cc, lc, 2, kL, tr.
+                iSplitL. iPureIntro.
+                  destruct (length cc); constructor; clear H6 H0;
+                  invert_all_in; (lia || list_elem_of).
+                doneL.
+                iFrame "#".
+                iSplit. iApply (big_sepL2_mono with "Htrtr"). by auto.
+                done.
+              ** iApply (big_sepL2_mono with "Htr'"). by auto.
+              ** iApply (big_sepL2_mono with "Hrtr"). by auto.
+              ** iPureIntro.
+                rewrite Hoeq Hleq !concat_app /=.
+                aac_rewrite Hnoeq.
+                aac_reflexivity.
+        Opaque isSpecialTriple.
+        * Transparent isNotSpecialTriple.
+          (* appeler la spec de pop_case_1_not_special *)
+          rewrite /prepare_pop_case_1.
+          iDestruct "Ht" as (fi c la fc cc lc kF kL tr) "(%tconf & -> & #Hfi & #Hc & #Hla & #Htrtr & %Hleq)".
+          wp_pures.
+          wp_apply (bhas_length_3_spec with "Hfi") as "_".
+          inversion tconf; wp_pures.
+          wp_apply (bconcat32_spec with "[Hp Hm]") as (b') "Hb'". by iFrame "#".
+          rewrite !isDeque_unfold.
+          iDestruct "Hc" as "[[-> ->] | (%ℓ' & -> & Hℓ')]".
+          2: {
+            do 2 wp_pure.
+            wp_bind (_ = _)%E.
+            iInv "Hℓ'" as "(%v' & Hv' & Hℓ'')".
+            wp_pure.
+            iExFalso.
+            iDestruct "Hv'" as (pr' ld' md' rd' sf' pc' lc' mc' rc' sc' kp' km' ks' lt rt) "(_ & %conf' & _ & _ & _ & _ & Hs' & _ & _ & ->)".
+            iDestruct (big_sepL2_length with "Htrtr") as "%Hlen".
+            rewrite Hlen in H8.
+            iDestruct (buffer_length with "Hs'") as "%Hslen".
+            assert (ks' > 0) as Hslen' by (inversion conf'; invert_all_in; lia).
+            rewrite !length_app in H8.
+            lia.
+          }
+          wp_pures.
+          wp_apply (bis_empty_spec with "Hla") as "_".
+          wp_pures.
+          iModIntro. iApply "Hψ".
+          iExists b', d', m, r, s, (op ++ fc), os', om, or, os,
+            5, 2, kSf, ltr', rtr.
+          rewrite -!isDeque_unfold.
+          doneL.
+          iSplit. iPureIntro. by easy_config.
+          iFrame "#". iFrame.
+          iSplit. iApply (big_sepL2_mono with "Htr'"). by auto.
+          iSplit. iApply (big_sepL2_mono with "Hrtr"). by auto.
+          destruct lc; [| iDestruct (buffer_length with "Hla") as "%No"; by inversion No ].
+          destruct cc; [| by inversion H6 ].
+          iPureIntro.
+          rewrite Hoeq Hleq /= app_nil_r.
+          aac_reflexivity.
+        Opaque isNotSpecialTriple.
+    Qed.
+
+  Global Instance isPopFiveTuplePersistent o d : Persistent (isPopFiveTuple o d).
+  Proof.
+    rewrite /isPopFiveTuple.
+    repeat (apply bi.exist_persistent; intro).
+    repeat (apply bi.sep_persistent; apply _).
+  Qed.
+
+End lemmas.
+
